src/Prototype/Reduction.v
@@ -9,86 +9,10 @@ Section Reduction.
   Local Notation MsgId := (MsgId MsgT).
   Local Notation Label := (Label MsgT).
 
-  (** Utilities end *)
-
   Definition Reduced (from to: list Label) (lbl1 lbl2: Label) :=
     exists hst1 hst2,
       from = hst1 ++ lbl1 :: lbl2 :: hst2 /\
       to = hst1 ++ lbl2 :: lbl1 :: hst2.
-
-  Lemma reduction_preserves_steps'':
-    forall lbl1 lbl2: Label,
-      msgTo (lbl_in lbl1) <> msgFrom (lbl_in lbl2) ->
-      msgTo (lbl_in lbl1) <> msgTo (lbl_in lbl2) ->
-      forall (obs: Objects MsgT StateT) oss1 oims1 oss2 oims2 hst,
-        steps obs oss1 oims1 (lbl1 :: lbl2 :: hst) oss2 oims2 ->
-        steps obs oss1 oims1 (lbl2 :: lbl1 :: hst) oss2 oims2.
-  Proof.
-    intros.
-    inv H1; inv H6.
-    inv H9; inv H10.
-
-    simpl in *.
-    pose proof (step_obj_idx H6).
-    pose proof (step_obj_idx H11).
-    rewrite H7, H10 in H0.
-
-    rewrite idx_add_comm by assumption.
-    rewrite <-distributeMsgs_idx_add_comm; [|exact StateT|auto].
-    rewrite distributeMsgs_comm by assumption.
-    rewrite idx_add_comm with (k1 := obj_idx obj) by assumption.
-    rewrite distributeMsgs_idx_add_comm; [|exact StateT|assumption].
-
-    econstructor; [econstructor|]; try eassumption; clear H5.
-    - econstructor.
-      + exact H1.
-      + reflexivity.
-      + rewrite find_idx_add_neq in H3 by assumption.
-        eassumption.
-      + rewrite find_distributeMsgs_neq in H4 by assumption.
-        rewrite find_idx_add_neq in H4 by assumption.
-        eassumption.
-      + eassumption.
-      + reflexivity.
-    - econstructor.
-      + exact H2.
-      + reflexivity.
-      + rewrite find_idx_add_neq by auto.
-        eassumption.
-      + rewrite find_distributeMsgs_neq by auto.
-        rewrite find_idx_add_neq by auto.
-        eassumption.
-      + eassumption.
-      + reflexivity.
-  Qed.
-  
-  Lemma reduction_preserves_steps':
-    forall lbl1 lbl2: Label,
-      msgTo (lbl_in lbl1) <> msgFrom (lbl_in lbl2) ->
-      msgTo (lbl_in lbl1) <> msgTo (lbl_in lbl2) ->
-      forall (obs: Objects MsgT StateT) hst1 oss1 oims1 oss2 oims2 hst2,
-        steps obs oss1 oims1 (hst1 ++ lbl1 :: lbl2 :: hst2) oss2 oims2 ->
-        steps obs oss1 oims1 (hst1 ++ lbl2 :: lbl1 :: hst2) oss2 oims2.
-  Proof.
-    induction hst1; simpl; intros.
-    - apply reduction_preserves_steps''; auto.
-    - inversion_clear H1.
-      econstructor; eauto.
-  Qed.
-
-  Theorem reduction_preserves_steps:
-    forall (obs: Objects MsgT StateT) oss1 oims1 hst oss2 oims2,
-      steps obs oss1 oims1 hst oss2 oims2 ->
-      forall lbl1 lbl2 hst',
-        Reduced hst hst' lbl1 lbl2 ->
-        msgTo (lbl_in lbl1) <> msgFrom (lbl_in lbl2) ->
-        msgTo (lbl_in lbl1) <> msgTo (lbl_in lbl2) ->
-        steps obs oss1 oims1 hst' oss2 oims2.
-  Proof.
-    unfold Reduced; intros.
-    destruct H0 as [hst1 [hst2 [? ?]]]; subst.
-    apply reduction_preserves_steps'; auto.
-  Qed.
 
 End Reduction.
         
